

$\textsection$ 1
1) 
1)$\int \frac{dx}{(x+1)(x-2)} = |\frac{1}{(x+1)(x-2)}=\frac{A}{(x+1)}+\frac{B}{(x-2)}|=|1=Ax-2A+Bx+B|=|A=\frac{1}{3},B=-\frac{1}{3}|=\int \frac{1}{3(x+1)}-\int \frac{1}{3(x-2)}=\frac{1}{3} (ln|x+1|-ln|x-2|)$
2)$\int \frac{xdx}{2x^2-3x-2} = \int \frac{xdx}{2(x-2)(x+\frac{1}{2})}=|\frac{x}{(x-2)(2x+1)}=\frac{A}{(x--2)}+\frac{B}{(2x+1)}|=|A=\frac{2}{5},B=\frac{1}{5}|=\int \frac{2}{5(x-2)}+\int \frac{1}{5(2x+1)}=\frac{2 ln|x-2|}{5}+\frac{1 ln|2x+1|}{10}$
3)$\int \frac{(2x+11)dx}{x^2+6x+13}=\int \frac{(2x+6)dx}{x^2+6x+13}+5\int \frac{dx}{(x+3)^2+4}=|\frac{u=x^2+6x+13 , t=x+3}{du=(2x+6)dx, dt=dx}|=\int \frac{du}{u}+5\int \frac{dt}{t^2+4}=ln|x^2+6x+13|+5\int \frac{dx}{4(\frac{x^2}{4}+1)}=ln|x^2+6x+13|+\frac{5}{2}(tg^{-1}(\frac{x+3}{2}))$
4)$\int \frac{(x^2-5x+9)dx}{x^2-5x+6}=x+3\int \frac{dx}{x-3}-3\int \frac{dx}{x-2}=x+3(ln|\frac{x-3}{x-2}|)$
5)$\int \frac{(3x^3-5x+8)dx}{x^2-4}=\int 3xdx+\int (\frac{17x+8}{x^2-4})dx=|\frac{17x+8}{x^2-4}=\frac{A}{x-2}+\frac{B}{x+2}|=|A=\frac{21}{2},B=\frac{13}{2}|=\frac{3x^2}{2}+\frac{21 ln|x-2|}{2}+\frac{13 ln|x+2|}{2}$
6)$\int \frac{x^2dx}{x^2-6x+10}=2\int \frac{(3x-5)dx}{x^2-6x+10}+x=\frac{3}{2}\int \frac{2x-6}{x^2-6x+10}+4\int \frac{dx}{x^2-6x+10}=\frac{3 ln|x^2-6x+10|}{2}-4 tg^{-1}(3-x)$
2) (ч)
2)$\int \frac{(2x^2+41x-91)dx}{(x-1)(x+3)(x-4)}=|\frac{2x^2+41x-91}{(x-1)(x+3)(x-4)}=\frac{A}{x-1}+\frac{B}{x+3}+\frac{C}{x-4}=|A=4,B=-7,C=5|=4 ln|x-1|-7|x+3|+5ln|x-4|$
4)$\int \frac{(5x-3)dx}{(x-2)(3x^2+2x-1)}=\int \frac{(5x-3)dx}{3(x-2)(x+1)(3x-1)}=|\frac{(5x-3)}{3(x-2)(x+1)(3x-1)}=\frac{A}{x-2}+\frac{B}{x+1}+\frac{C}{3x-1}=|A=\frac{7}{15},B=-\frac{2}{3},C=\frac{3}{5}|=\frac{7}{45}ln|x-2|-\frac{2}{3}ln|x+1|+\frac{1}{5}ln|3x-1|$
6)$\int \frac{(5x-14)dx}{(x^3-x^2-4x+4)}=\int \frac{(5x-14)dx}{(x-2)(x+2)(x-1)}=|\frac{(5x-14)}{(x-2)(x+2)(x-1)}=\frac{A}{x-2}+\frac{B}{x+2}+\frac{C}{x-1}=|A=-1,B=-2,C=3|=-ln|x-2|-2ln|x+2|+3ln|x-1|$
8)$\int \frac{(x^2+1)dx}{(x^2-1)(x^2-4)}=\int \frac{(x^2+1)dx}{(x-1)(x+1)(x+2)(x-2)}=|\frac{(x^2+1)dx}{(x-1)(x+1)(x+2)(x-2)}=\frac{A}{(x-2)}+\frac{B}{x+2}+\frac{C}{x-1}+\frac{D}{x+1}=|A=5/12,B=-5/12,C=-1/3, D=1/3|=-\frac{5}{12}ln|x-2|+\frac{5}{12}ln|x+2|-\frac{1}{3}ln|x-1|+\frac{1}{3}ln|x+1|+C$
10)$\int \frac{(x^6-2x^4+3x^3-9x^2+4)dx}{(x^5-5x^3+4x)}=\int xdx + \int \frac{(3x^4-x^3-9x^2+4)dx}{x(x^4-5x^2+4)}=\frac{x^2}{2}+\frac{A}{x}+\frac{B}{x-1}+\frac{C}{x+1}+\frac{D}{x-2}+\frac{E}{x+2}=|A=1,B=\frac{1}{2},C=\frac{3}{2},D=1,E=-1|=\frac{x^2}{2}+ln|\frac{x(x-2)}{x+2}|+\frac{1}{2}ln|x-1|+\frac{3}{2}ln|x+1|$

1) 
1)$\int \frac{x\sqrt{x}}{1+\sqrt{x}}=|\frac{u=\sqrt{x}}{du=\frac{dx}{2\sqrt{x]}}}|=2\int \frac{u^4du}{u+1}=\int(u^3-u^2+u+\frac{1}{u+1}-1)du=\frac{u^4}{4}-\frac{u^3}{3}+\frac{u^2}{2}-u+ln|1+u|=\frac{x^2}{4}-\frac{x^\frac{3}{2}}{3}+\frac{x}{2}-\sqrt{x}+ln|1+\sqrt{x}|+C$
2)$\int (\frac{1-2\sqrt{x})dx}{1+2\sqrt{x}}=|\frac{u=\sqrt{x}}{du=\frac{1}{2\sqrt{x}}}|=2\int \frac{u-2u^2)du}{2u+1}=2\int (1-u-\frac{1}{2u+1})du=2(u-\frac{u^2}{2}-\frac{ln|2u+1|}{2})=2\sqrt{x}-x-\frac{ln|2\sqrt{x}+1|}{2}+C$
3)$\int (\frac{\sqrt{x+1}+1)dx}{\sqrt{x+1}-1}=|\frac{u=x+1}{du=dx}|=\int \frac{(\sqrt{u}+1)du}{\sqrt{u}-1}=|\frac{s=\sqrt{u}}{ds=\frac{du}{2\sqrt{u}}}|=2\int \frac{s(s+1)ds}{s-1}=2\int(s+2+\frac{2}{s-1})ds=(x+1)+2\sqrt{x+1}+4ln|\sqrt{x+1}-1|+C$
6)$\int \frac{xdx}{\sqrt[4]{x^3(4-x)}}=\int \frac{dx}{\sqrt{\frac{4}{x}-1}}=|\frac{u=\frac{1}{x}}{du=-\frac{1}{x^2}}|=-\int\frac{du}{u^2\sqrt{4u-1}}=|\frac{t=4u-1}{dt=4du}|=-4\int \frac{dt}{(t+1)^2\sqrt{t}}=|\frac{s=\sqrt{t}}{ds=\frac{dt}{2\sqrt{t}}}|=-8\int \frac{ds}{(s^2+1)^2}=|\frac{s=tg(w)}{ds=sec^2(w)dw}|=-8\int cos^2(w)dw=-4\int (cos(2w)+1)dw = -4(sin(arctg(\sqrt{\frac{4}{x}-1}))cos(arctg(\sqrt{\frac{4}{x}-1}))+arctg(\sqrt{\frac{4}{x}-1}))$
Ссылки: [[2 практика матан БТ]]
