1.2) $(\frac{\partial P}{\partial V})_T  = -\frac{1}{\beta V}$
$(\frac{\partial V}{\partial T})_P  = \alpha V_0$
$(\frac{\partial T}{\partial P})_V  = \frac{1}{\gamma V} \rightarrow V_0\alpha = p_0V\gamma\beta$ 

1.7) $\beta = -\frac{1}{V}(\frac{\partial V}{\partial P})_T , \rho = \frac{m}{V} | d \rightarrow$
$0 = d\rho V + \rho dV \rightarrow dV = -V\frac{d\rho}{\rho}$
$\beta = \frac{1}{\rho}(\frac{\partial \rho}{\partial P})_T \rightarrow \frac{\partial \rho}{\partial P} = \rho \beta ; \beta << 1 \rightarrow \rho ~ const \rightarrow \frac{\Delta \rho}{\Delta P} ~ (\frac{\partial \rho}{\partial P})_T = \rho \beta$
$\rho - \rho_0 = \Delta p \rho_0 \beta \rightarrow \rho = \rho_0(1+\beta \Delta p)$ ...

1.12) $\frac{1}{V_0}(\frac{\partial V}{\partial T})_P  = \alpha \rightarrow (\frac{\partial V}{\partial T})_P = const$
$V = V_0 + (\frac{\partial V}{\partial T})_P(T-T_0) = V_0(1+\alpha(T-T_0))$
$\rho = \rho_0(1+\alpha(T-T_0))^{-1}$
$M_1 = \rho_1 V , M_2 = \rho_2 V \rightarrow \Delta M = V(\rho_2 - \rho_1)$
$\rightarrow V\rho_0 (\frac{1}{(1+\alpha t_1)} - \frac{1}{(1+\alpha t_2)})$

1.14) $P = \frac{3mRT}{4\pi R_0^{3} \mu}$
$F_{давл} = p\cdot\pi R_0^{2}$
$p\cdot\pi R_0^{2} = \sigma2\pi R_0d$
$p = \frac{2d\sigma}{R_0}$
$m = \frac{4p\pi \mu R_0^{3}}{RT} = \frac{2\mu \sigma m_{*}}{3RT \rho_{*}}$

1.26) 
1) $Q_{13} = \Delta U_{13} , Q_{32} = \Delta U_{32}+A_{32}$
$Q_{132} = \Delta U_{13}+U_{32}+A_{32} = 0 \rightarrow \Delta U_{132} = Q_{132} = Q_{132}-A_{32}$
2)  $Q_{14} = \Delta U_{14} , Q_{42} = \Delta U_{42}$
$Q_{142} = \Delta U_{14}+U_{132} = A_{142} + Q_{132}-A_{132}$
...

1.45) $U = f(T) , \delta Q = dU+pdV$
$V - const \rightarrow \delta Q  = dU$
$C_V = \frac{dU}{dT} = const \rightarrow u = c_VT$ , при политропическом процессе $c_V = const$
$(c-c_V)dT = \frac{\nu RT}{V}dV$
$(c-c_V)d(lnT) - \nu R ln(V)) = 0$
$d((c-c_V)lnT - \nu R ln(V)) = 0$
$T^{c-c_V}V^{-\nu R} = const <-> TV^{-\frac{\nu R}{c-c_V}} = const$
$PV^{1-\frac{\nu R}{c-c_V}} = const \rightarrow PV^{\frac{c-c_p}{c-c_V}} = const$
1) $V \uparrow \rightarrow T \downarrow$
2) $2 = \frac{c-c_p}{c-c_V} = \frac{c_{\mu}-c_{p \mu}}{c_{\mu}-c_{V \mu}} \rightarrow c_{\mu} = c_{V \mu}-R$

1.50)  $c_{\mu} = c_{o \mu}+\alpha T$
$\delta Q = dU+pdV$
$(c_{V \mu}+\alpha T) \nu dT = c_{V \mu}\nu dT + \frac{\nu RTdV}{V}$
$\frac{(c_{o \mu}+\alpha T - C_{V\mu})dT}{T} = R\frac{dV}{V}$
$(c_{o \mu} - C_{V\mu})d(lnT)+\alpha dT - Rd(lnV) = 0$
$T^{(c_{o \mu} - C_{V\mu})}e^{\alpha T}V^{-R} = const$

1.58) $PV^{\gamma} = const , Q=const \rightarrow c = 0 \rightarrow \gamma = \frac{c_p}{c_v}$(адиабатический)
$Q_1 = c_p(T_2-T_1) =  c_p(3T)$
$Q_2 = c_v(T_4-T_3) = c_v(4T)$
$\gamma = \frac{c_p}{c_v} = \frac{4}{3}$

![[Снимок экрана от 2024-02-26 09-21-07.png]]
![[Снимок экрана от 2024-02-26 09-21-13.png]]
![[Снимок экрана от 2024-02-26 09-21-47.png]]![[Снимок экрана от 2024-02-26 09-22-05.png]]
![[Снимок экрана от 2024-02-26 09-22-21.png]]
![[Снимок экрана от 2024-02-26 09-22-32.png]]
![[Снимок экрана от 2024-02-26 09-22-52.png]]
![[Снимок экрана от 2024-02-26 09-23-03.png]]
![[Снимок экрана от 2024-02-26 09-23-30.png]]
![[Снимок экрана от 2024-02-26 09-24-14.png]]
![[photo_2024-02-26_04-40-41 (2).jpg]]![[photo_2024-02-26_04-40-42.jpg]]
![[photo_2024-02-26_04-40-42 (2).jpg]]![[photo_2024-02-26_04-40-43.jpg]]
![[photo_2024-02-26_04-40-44.jpg]]
![[photo_2024-02-26_04-40-44 (2).jpg]]
![[photo_2024-02-26_04-40-45.jpg]]![[photo_2024-02-26_04-40-47.jpg]]
![[photo_2024-02-26_04-40-47 (2).jpg]]
Ссылки: [[1-3 лекции физика БТ]]
