---
cssclasses:
---

1) $\int e^{-\frac{1}{x}}\frac{dx}{x} = \bigl[ \frac {t = -\frac{1}{x^2}}{dx = -\frac{2dx}{x^3}} \bigr] = \int e^{t}\frac{dt}{2} = \frac{1}{2} e^{-\frac{1}{x^2}} + c$
2) $\int \frac{dx}{sinx} = \int \frac{dx}{2sin\frac{x}{2}cos\frac{x}{2}} = \int \frac{cos\frac{x}{2}}{2sin\frac{x}{2}cos^2\frac{x}{2}} = \bigl[ \frac{t = tg\frac{x}{2}}{dt = \frac{1}{2}\frac{1}{cos^2\frac{x}{2}}} \bigr] = \int t^{-1}dt = ln|t|+C = ln|tg\frac{x}{2}|+C$
3) $\int \sqrt{a^2 + x^2}dx = \bigl[ \frac{x = acost}{dx = -asindt} \bigr] = -\int \sqrt{a^2-a^2cos^2t}\space a sintdt = \int -\sqrt{a^2sin^2t}\space asintdt = -\int a^2sin^2tdt = \int a^2 \frac{1-cos2t}{2}dt = \frac{a^2t}{2} - \frac{a^2 \sin{2t}}{4} = \frac{a^2}{2}(arccos\frac{x}{a} - \frac{sin(2arccos\frac{x}{a})}{2}) + C$

4) $\int \sqrt{a^2+x^2}dx = \bigl[ \frac{x = asinh(t)}{dx = acosh(t)dt} \bigr] = \int a\sqrt{a^2 + a^2 sinh^2(t)}dt = a^2 \sqrt{1+sinh^2t}dt = a^2 \int cosh^2tdt = \frac{1+cosh2t}{2} = \frac{a^2}{2} \int (1+cosh2t)dt = \frac{a^2}{2}(t+\frac{sinh(2t)}{2}) + C$
5) $\int xcosxdx = \int xd(sinx) = xsinx - \int sinxdx = xsinx+cosx+C$
6) $\int arctgxdx = xarctgx-\int \frac{xdx}{1+x^2} = xarctgx - \frac{1}{2}\int \frac{d(1+x^2)}{1+x^2} = xarctgx - \frac{1}{2}ln|1+x^2|+C$
7) $\int xarctgx \space dx = \int arctgx d(\frac{x^2}{2}) = \frac{x^2arctgx}{2} - \int \frac{x^2d(arctgx)}{2} = \frac{x^2arctgx}{2} - \int \frac{x^2dx}{2(x^2+1)} = \frac{x^2arctgx}{2} - (\frac{x-arctgx}{2})$
8) $\int e^x cosxdx = \int e^xd(sinx) = e^xsinx - \int sinx e^xcosx = e^xsinx+e^xcosx - \int e^xcosxdx = 2\int e^xcosxdx = e^x(sinx+cosx) \rightarrow \int e^x cosxdx = \frac{e^x}{2}(sinx+cosx) + C$
9) $\int \frac{x^2+1}{(x-1)^3 (x+3)}$
$\frac{x^2+1}{(x-1)^3(x+3)} = \frac{A}{x+3} + \frac{B}{x-1} + \frac{C}{(x-1)^2} + \frac{D}{(x-1)^3}$
$A = -\frac{5}{32} , B = \frac{5}{32} , C = \frac{3}{8} , D = \frac{1}{2}$
= $\int (\frac{-5}{32(x+3)} + \frac{5}{32(x-1)} + \frac{3}{8(x-1)^2} + \frac{1}{2(x-1)^3})dx = ...$
10) $\int \frac{(3x+4)dx}{\sqrt{-x^2+6x+8}} = -\frac{3}{2} \int \frac{(-2x-\frac{8}{3}+6-6)dx}{\sqrt{-x^2+6x+8}} = -\frac{3}{2} \int \frac{d(-x^2+6x+8)}{\sqrt{-x^2+6x+8}} + B(\int \frac{dx}{\sqrt{-x^2+6x+8}})= -3\sqrt{-x^2+6x+8} + Barcsin\frac{x-3}{\sqrt{17}} + C$
11) $\int \frac{dx}{x\sqrt{5x^2-2x+1}} = \bigl[ \frac{t = \frac{1}{x}}{dt = -\frac{dx}{x^2}} \bigr] = -\int \frac{dt}{\sqrt{t^2-2t+3}} = -\int \frac{dt}{\sqrt{t^2-2t+3}} = -\int \frac{dt}{\sqrt{(t-1)^2+1}} = -ln|t-1+\sqrt{(t-1)^2+4}| + C$

Ссылки: [[1 практика матан БТ]]
[[2 лекция матан БТ]]
